Try to remove axiom1 after F* update; Add Makefile

Free.fst
@@ -9,21 +9,17 @@ type cmd_sig (op:Type u#a) = {
 }
 
 noeq
-type freef op (s : cmd_sig op) a =
-  | Call : (l:op) -> (s.args l) -> (maybe (s.res l) -> a) -> freef op s a
-
-val freef_fmap : (#a:Type) -> (#b:Type) -> (#op:Type) -> (#s:cmd_sig op) ->
-                m:freef op s a -> (x:a{x<<m} -> b) -> freef op s b
-let freef_fmap #a #b #op #s m f=
-  match m with
-  | Call cmd args fnc -> Call cmd args (fun i -> FStar.WellFounded.axiom1 fnc i; f (fnc i))
-
-noeq
 type free (op:Type u#o) (s:cmd_sig op) (a:Type u#a) : Type u#(max o a) =
-  | Cont : freef op s (free op s a) -> free op s a
+  | Call : (l:op) -> (s.args l) -> cont:(maybe (s.res l) -> (free op s a)) -> free op s a
   | Return : a -> free op s a
   // TODO: is this relevant? can be made a silent cmd
   | Throw : exn -> free op s a
+
+let free_codomain_ordering (#op:Type) (#s:cmd_sig op) (#a:Type) (x:(free op s a){Call? x})
+  : Lemma (forall r. Call?.cont x r << x)
+  = ()
+
+
 
 let free_return (op:Type) (s:cmd_sig op) (a:Type) (x:a)   : free op s a = Return x
 let free_throw  (op:Type) (s:cmd_sig op) (a:Type) (x:exn) : free op s a = Throw x 
@@ -32,8 +28,9 @@ let rec free_bind (op:Type u#o) (s:cmd_sig op) (a:Type u#a) (b:Type u#b) (l : fr
   match l with
   | Return x -> k x 
   | Throw err -> Throw err 
-  | Cont t -> Cont (freef_fmap t (fun fnci ->
-      free_bind op s a b fnci k))
+  | Call cmd args fnc -> 
+      Call cmd args (fun i ->
+        free_bind op s a b (fnc i) k)
 
 val lift_error : (#op:Type) -> (#s:cmd_sig op) -> (#a:Type) -> (maybe a) -> free op s a
 let lift_error #op #s #a v =
@@ -41,10 +38,10 @@ let lift_error #op #s #a v =
   | Inl x -> free_return op s a x
   | Inr err -> free_throw op s a err
 
-val free_perform : (#op:Type) -> (#s:cmd_sig op) -> (#a:Type) -> freef op s (maybe a) -> free op s a
+val free_perform : (#op:Type) -> (#s:cmd_sig op) -> (#a:Type) -> free op s (maybe a) -> free op s a
 let free_perform #op #s #a v = 
   free_bind op s (maybe a) (a) 
-    (Cont (freef_fmap #(maybe a) #_ v Return))
+    v
     lift_error
 
 let free_map (op:Type u#o) (s:cmd_sig op) (a:Type u#a) (b:Type u#b) (l : free op s a) (k : a -> b) : free op s b =
